theories/Data/FiniteMap.v
@@ -30,10 +30,6 @@ Universe U_alist_key.
 
 Universe U_alist_val.
 
-Constraint U_alist_key = alist.u0.
-
-Constraint U_alist_val = alist.u1.
-
 #[global]
 Instance alist_is_similar_to_option_kleisli {K : Type@{U_alist_key}} {V : Type@{U_alist_val}} {V' : Type@{U_alist_val}} (Sim_V_V' : Similarity V V') : Similarity (alist K V) (K -> option V') :=
   fun m => fun m' => forall k : K, forall v : V, forall v' : V', forall v_sim_v' : v =~= v', (k, v) ∈ kvlist m <-> m' k = Some v'.
@@ -492,7 +488,7 @@ Instance fpmap_hsOrd : hsOrd (fpmap K V) (PROSET := Poset_isProset) :=
 Next Obligation.
   intros m m' OBS_Lt. pose proof (compare_Lt m.(FinitePartialMap.data) m'.(FinitePartialMap.data) OBS_Lt) as [LE NE]. split.
   - exact LE.
-  - intros m_eq_m'. contradiction NE. do 6 red in m_eq_m' |- *.
+  - intros m_eq_m'. contradiction NE. cbn in m_eq_m' |- *.
     rewrite -> FinitePartialMap.t_eq_iff in m_eq_m'. rewrite m_eq_m'. reflexivity.
 Qed.
 Next Obligation.
@@ -502,7 +498,7 @@ Qed.
 Next Obligation.
   intros m m' OBS_Gt. pose proof (compare_Gt m.(FinitePartialMap.data) m'.(FinitePartialMap.data) OBS_Gt) as [LE NE]. split.
   - exact LE.
-  - intros m_eq_m'. contradiction NE. do 6 red in m_eq_m' |- *.
+  - intros m_eq_m'. contradiction NE. cbn in m_eq_m' |- *.
     rewrite -> FinitePartialMap.t_eq_iff in m_eq_m'. rewrite m_eq_m'. reflexivity.
 Qed.
 
